\documentclass{article}

\usepackage[utf8]{inputenc}
\usepackage{mathtools}
\usepackage{listings}
\usepackage{color}
\usepackage{fancyvrb}
\usepackage{tabularx}
\usepackage{fancyref}
\usepackage{enumitem}
\usepackage[margin=0.75in]{geometry}
\usepackage{amsmath}
\usepackage[square,numbers,sort&compress]{natbib}

\title{Molecular Simulation of Materials, Homework 2}
\author{Matthew Grasinger}

\begin{document}

\lstset{language=C++,
        basicstyle=\ttfamily,
        keywordstyle=\color{blue}\ttfamily,
        stringstyle=\color{red}\ttfamily,
        commentstyle=\color{green}\ttfamily,
        morecomment=[l][\color{magenta}]{\#},
        breaklines=true,
        postbreak=\raisebox{0ex}[0ex][0ex]{\ensuremath{\color{red}\hookrightarrow\space}}
}

\pagenumbering{gobble}
\vspace{3.5in}
\maketitle
\clearpage
\pagenumbering{arabic}

\newcommand{\p}{\mathbf{p}}
\newcommand{\pos}{\mathbf{r}}

\section{Problem 1}

\begin{enumerate}[label=\alph*)]
  \item \begin{enumerate}[label=\roman*]
      \item \begin{align*}
          \frac{1}{2m_i} \frac{\partial |\p_i|^2}{\partial \p_i} = & \frac{1}{2m_i} \frac{\partial \left[\p_i \cdot \p_i\right]}{\partial \p_i}, \\
          = & \frac{1}{2m_i} \frac{\partial \left[p_{i1}^2 + p_{i2}^2 + p_{i3}^2\right]}{\partial p_{ij}}, \\
        = & \frac{1}{2m_i} \begin{Bmatrix}2p_{i1} \\ 2p_{i2} \\ 2p_{i3}\end{Bmatrix}, \\
        = & \frac{2 \p_i}{2m_i}, \\
        = & \frac{\p_i}{m_i}.
        \end{align*}
      \item \begin{align*}
          \frac{\partial r_{ij}}{\partial \pos_i} = & \frac{\partial \sqrt{\left(r_{i1} - r_{j1}\right)^2 + \left(r_{i2} - r_{j2}\right)^2 + \left(r_{i3} - r_{j3}\right)^2}}{\partial \pos_i}, \\
        = & \begin{Bmatrix} \frac{1}{2} \left[\left(r_{i1} - r_{j1}\right)^2 + \left(r_{i2} - r_{j2}\right)^2 + \left(r_{i3} - r_{j3}\right)^2\right]^{-1/2} 2\left(r_{i1} - r_{j1}\right) \\ \frac{1}{2} \left[\left(r_{i1} - r_{j1}\right)^2 + \left(r_{i2} - r_{j2}\right)^2 + \left(r_{i3} - r_{j3}\right)^2\right]^{-1/2} 2\left(r_{i2} - r_{j2}\right) \\ \frac{1}{2} \left[\left(r_{i1} - r_{j1}\right)^2 + \left(r_{i2} - r_{j2}\right)^2 + \left(r_{i3} - r_{j3}\right)^2\right]^{-1/2} 2\left(r_{i3} - r_{j3}\right) \end{Bmatrix}, \\
          = & \frac{1}{2} r_{ij}^{-1} 2\pos_{ij}, \\
          = & \frac{\pos_{ij}}{r_{ij}}.
        \end{align*}
      \item 
        \begin{align*}
          \mathcal{H} = & \mathcal{K} + \mathcal{U}, \\
          = & \Sigma_i \frac{\left|\p_i\right|^2}{2 m_i} + \mathcal{U}. \\
        \end{align*}
        TODO: FINISH THIS PROOF
    \end{enumerate}
  \item \begin{align*}
      v_{i,x}(t + \Delta t) & = v_{i,x}(t) + \frac{\partial v_{i,x}}{\partial t}\Bigr|_{t} (\Delta t) + \frac{1}{2} \frac{\partial^2 v_{i,x}}{\partial t^2}\Bigr|_{t} (\Delta t)^2, \\
                            & = v_{i,x}(t) + \frac{F_{i,x}(t)}{m_i} (\Delta t) + \frac{1}{2} \frac{\partial^2 v_{i,x}}{\partial t^2}\Bigr|_{t} (\Delta t)^2.
    \end{align*}
    Recall that $v_{i,x}(t + \Delta t / 2) = v_{i,x}(t) + F_{i,x}(t) \Delta t/(2m_i)$.
    \begin{equation} \label{eq:vi3}
      v_{i,x}(t + \Delta t) = v_{i,x}(t + \Delta t / 2) + \frac{F_{i,x}(t)}{2m_i}(\Delta t) + \frac{1}{2} \frac{\partial^2 v_{i,x}}{\partial t^2}\Bigr|_{t} (\Delta t)^2.
    \end{equation}
    We can simplify \eqref{eq:vi3} further by considering the Taylor expansion of the force:
    \begin{align}
    F_{i,x}(t + \Delta t) & = F_{i,x}(t) + \frac{\partial F_{i,x}}{\partial t}\Bigr|_{t} (\Delta t), \\
                          & = F_{i,x}(t) + \frac{\partial}{\partial t}\left[m_i \frac{\partial v_{i,x}}{\partial t}\right]\Bigr|_{t} (\Delta t), \\
      \label{eq:Ftaylor} & = F_{i,x}(t) + m_i \frac{\partial^2 v_{i,x}}{\partial t^2}\Bigr|_{t}(\Delta t).
    \end{align}
    Dividing both sides of \eqref{eq:Ftaylor} by $2m_i$ and plugging into \eqref{eq:vi3} yields the desired result.
\end{enumerate}

\end{document}
